src/proof/simplereplicaset.v
@@ -54,10 +54,12 @@ Lemma wp_manageReplicas γ l (gv: schema.GroupVersion.t) pod_l_sl rs_l
       "Hghostown_children" ∷ rs_key [[ γ.(γ_children) ]]↦ dom pure_pod_map ∗
       "Hghostown_grandchildren" ∷ ([∗ map] key ↦ s ∈ grand_child_keys, key [[ γ.(γ_children) ]]↦ s) ∗
       "%Hdom_eq" ∷ ⌜ dom pure_pod_map = dom grand_child_keys ⌝ ∗
-      "%Hagree_with_keys" ∷ ⌜ ∀ key pod, pure_pod_map !! key = Some pod → PureKObject.agree_with_key key (PureKObject.Pod pod) ⌝ ∗
+      "%Hpods_keys_eq" ∷ ⌜ ∀ key pod, pure_pod_map !! key = Some pod → key = PurePod.key pod ⌝ ∗
+      "%Hpods_ns_eq" ∷ ⌜ ∀ key, key ∈ dom pure_pod_map → key.(KKey.Namespace') = rs_key.(KKey.Namespace') ⌝ ∗
       "%Hactive_map_eq" ∷ ⌜ active_pure_pod_map = filter (λ kv, controller.is_pure_pod_active (snd kv)) pure_pod_map ⌝ ∗
       "%Hlen_size" ∷ ⌜ size active_pure_pod_map = sint.nat (slice.len_f pod_l_sl) ⌝ ∗
-      "%Hin" ∷ ⌜ ∀ pure_pod, pure_pod ∈ active_pure_pods → ∃ k, active_pure_pod_map !! k = Some pure_pod ⌝ ∗
+      "%Hin" ∷ ⌜ ∀ pure_pod, pure_pod ∈ active_pure_pods → active_pure_pod_map !! (PurePod.key pure_pod) = Some pure_pod ⌝ ∗
+      "%Hunique" ∷ ⌜ ∀ i j p1 p2, active_pure_pods !! i = Some p1 → active_pure_pods !! j = Some p2 → (PurePod.key p1) = (PurePod.key p2) → i = j ⌝ ∗
       "%Hreplicas_eq" ∷ ⌜ pure_rs.(PureReplicaSet.Spec').(PureReplicaSetSpec.Replicas') = Some n ⌝
   }}}
   @! simplereplicaset.manageReplicas #pod_l_sl #rs_l
@@ -71,12 +73,28 @@ Lemma wp_manageReplicas γ l (gv: schema.GroupVersion.t) pod_l_sl rs_l
   }}}.
 Proof.
   wp_start as "H". iNamed "H". iDestruct "Hdeepown_l_rs" as "(Hrs_l & Hdeepown_rs)".
+  iDestruct (own_slice_len with "Hpod_l_sl") as %(Hpod_l_sl_len1 & Hpod_l_sl_len2).
+  iDestruct (own_slice_wf with "Hpod_l_sl") as %Hpod_l_sl_cap.
+  iDestruct (big_sepL2_length with "Hptrs") as %Hlen1.
+  iDestruct (big_sepL2_length with "Hdeepown_pods") as %Hlen2.
+  assert (length active_pure_pods = size (filter (λ kv : KKey.t * PurePod.t, is_pure_pod_active kv.2) pure_pod_map)) as Hlen_size_eq.
+  { congruence. }
+  assert (∀ i j p1 p2, i ≠ j → active_pure_pods !! i = Some p1 → active_pure_pods !! j = Some p2 → (PurePod.key p1) ≠ (PurePod.key p2)) as Hno_dup.
+  { intros i0 j p1 p2 Hneq Hlookup_i Hlookup_j Heq_key.
+    assert (p1 ∈ active_pure_pods) as Hin_p1 by (eapply list_elem_of_lookup_2; apply Hlookup_i).
+    assert (p2 ∈ active_pure_pods) as Hin_p2 by (eapply list_elem_of_lookup_2; apply Hlookup_j).
+    apply Hin in Hin_p1.
+    apply Hin in Hin_p2.
+    rewrite Heq_key in Hin_p1.
+    rewrite Hin_p1 in Hin_p2.
+    injection Hin_p2 as Heq_pods.
+    exfalso. apply Hneq.
+    eapply Hunique; eauto. }
   iDestruct (struct_fields_split with "Hrs_l") as "Hrs_l". iNamed "Hrs_l". wp_auto.
   iNamedPrefix "Hdeepown_rs" "Hrs_". iNamedPrefix "Hrs_Hdeepown_spec" "Hrs_".
   iAssert ((rs.(v1.ReplicaSet.Spec').(v1.ReplicaSetSpec.Replicas')↦{dq2}n)%I) with "[Hrs_Hdeepown_replicas_some]" as "Hreplicas".
   { rewrite Hreplicas_eq. iDestruct "Hrs_Hdeepown_replicas_some" as "(%replicas & Hreplicas & ->)". done. }
   wp_auto.
-  iDestruct (own_slice_len with "Hpod_l_sl") as %(Hpod_l_sl_len1 & Hpod_l_sl_len2).
   destruct Hpure_rs_well_formed as (Hpure_rs_meta_well_formed & Hpure_rs_spec_well_formed & _).
   destruct Hpure_rs_spec_well_formed as (Hpure_rs_spec_replicas_well_formed & Hpure_rs_spec_template_well_formed).
   assert (0 ≤ sint.Z n) as Hn.
@@ -143,34 +161,36 @@ Proof.
       }
       iFrame.
       iApply (struct_fields_combine (V:=v1.ReplicaSetSpec.t)). iFrame.
-    + iApply "HΦ". iFrame. iPureIntro. split.
-      * rewrite Hdom_eq'. done.
-      * rewrite Hpod_number'. word.
+    + iApply "HΦ". iFrame. iPureIntro. split. all: try done.
+      rewrite Hpod_number'. word.
   - wp_if_destruct.
     2: { iApply "HΦ". iFrame. iPureIntro. split.
       * rewrite Hdom_eq. done.
       * word. }
-    iDestruct (own_slice_len with "Hpod_l_sl") as %Hpod_l_sl_len.
-    iDestruct (own_slice_wf with "Hpod_l_sl") as %Hpod_l_sl_cap.
     wp_bind.
     wp_apply wp_slice_slice_pure; [iPureIntro;word|].
     iDestruct (own_slice_f 0 (word.sub (slice.len_f pod_l_sl) (W64 (sint.Z n))) with "Hpod_l_sl")
       as "(Hbefore_slice & Hslice & Hafter_slice )"; [word|].
     iDestruct (own_slice_len with "Hslice") as %(Hslice_len1 & Hslice_len2).
-    iDestruct (big_sepL2_length with "Hptrs") as %Hlen.
-    set I := (∃ (i: w64) (pod: loc) (pure_pod_map': gmap KKey.t PurePod.t) (grand_child_keys': gmap KKey.t (gset KKey.t)),
+    set I := (∃ (i: w64) (pod: loc) (pure_pod_map' active_pure_pod_map': gmap KKey.t PurePod.t) (grand_child_keys': gmap KKey.t (gset KKey.t)),
       "Hi_ptr" ∷ i_ptr ↦ i ∗
       "Hpod_ptr" ∷ pod_ptr ↦ pod ∗
       "Hghostown_pods" ∷ ([∗ map] key ↦ pod ∈ pure_pod_map', key [[ γ.(γ_state) ]]↦ PureKObject.Pod pod) ∗
       "Hghostown_children" ∷ rs_key [[ γ.(γ_children) ]]↦ dom pure_pod_map' ∗
       "Hghostown_grandchildren" ∷ ([∗ map] key ↦ s ∈ grand_child_keys', key [[ γ.(γ_children) ]]↦ s) ∗
       "%Hdom_eq'" ∷ ⌜ dom pure_pod_map' = dom grand_child_keys' ⌝ ∗
-      "%Hpod_number'" ∷ ⌜ size (filter (λ kv, controller.is_pure_pod_active (snd kv)) pure_pod_map') = Z.to_nat ((sint.Z (slice.len_f pod_l_sl)) + sint.Z i) ⌝ ∗
+      "%Hactive_map_eq'" ∷ ⌜ active_pure_pod_map' = filter (λ kv, controller.is_pure_pod_active (snd kv)) pure_pod_map' ⌝ ∗
+      "%Hpod_number'" ∷ ⌜ size active_pure_pod_map' = Z.to_nat ((sint.Z (slice.len_f pod_l_sl)) - sint.Z i) ⌝ ∗
+      "%Hin'" ∷ ⌜ ∀ pure_pod, pure_pod ∈ (drop (sint.nat i) active_pure_pods) →
+                                active_pure_pod_map' !! (PurePod.key pure_pod) = Some pure_pod ⌝ ∗
+      "%Hmap_sub" ∷ ⌜ ∀ pure_pod, pure_pod ∈ (drop (sint.nat i) active_pure_pods) →
+                                    pure_pod_map' !! (PurePod.key pure_pod) = Some pure_pod →
+                                      pure_pod_map !! (PurePod.key pure_pod) = Some pure_pod ⌝ ∗
       "%Hi" :: ⌜0 ≤ sint.Z i ≤ sint.Z (slice.len_f (slice.slice_f pod_l_sl ptrT (W64 0) (word.sub (slice.len_f pod_l_sl) (W64 (sint.Z n)))))⌝
     )%I.
     iAssert (I) with "[i pod Hghostown_pods Hghostown_children Hghostown_grandchildren]" as "Hloop_inv". {
-    iExists (W64 0), (default_val loc), pure_pod_map, grand_child_keys.
-    iFrame. iPureIntro. split_and!; [done|word|word|word]. }
+    iExists (W64 0), (default_val loc), pure_pod_map, (filter (λ kv : KKey.t * PurePod.t, is_pure_pod_active kv.2) pure_pod_map), grand_child_keys.
+    iFrame. iPureIntro. split_and!. all: try done. word. }
     wp_for "Hloop_inv". wp_if_destruct.
     + wp_pure; [rewrite /slice.slice_f /=;word|].
       set sliced_ptrs := (subslice (sint.nat (W64 0)) (sint.nat (word.sub (slice.len_f pod_l_sl) (W64 (sint.Z n)))) ptrs).
@@ -178,19 +198,173 @@ Proof.
       { rewrite Hslice_len1 /slice.slice_f /=. word. }
       wp_apply (wp_load_slice_elem with "[$Hslice]"); [word|eauto|].
       iIntros "Hslice". wp_auto.
-      wp_bind.
       assert (ptrs !! sint.nat i = Some this_ptr) as Hlookup_ptrs.
       { eapply lookup_take_Some in Hthis_ptr_lookup. intuition. }
       assert (∃ active_pod, active_pods !! sint.nat i = Some active_pod) as [active_pod Hlookup_active_pods].
-      { apply lookup_lt_is_Some_2. rewrite <-Hlen. word. }
-      iDestruct (big_sepL2_lookup with "Hptrs") as "Hthis_ptr".
+      { apply lookup_lt_is_Some_2. rewrite <-Hlen1. word. }
+      iDestruct (big_sepL2_lookup_acc with "Hptrs") as "[Hthis_ptr Hother_ptrs]".
       { apply Hlookup_ptrs. }
       { apply Hlookup_active_pods. }
       iDestruct (struct_fields_split with "Hthis_ptr") as "Hthis_ptr". iNamedPrefix "Hthis_ptr" "Hpod_". wp_auto.
       wp_apply wp_globals_get.
-      (* wp_apply (wp_State__PodDelete with "[$Hdeepown_l_this_pod $Hghostown_rs $Hghostown_children]").
-      { iFrame "#". iPureIntro. unfold PureObjectMeta.well_formed in Hpure_rs_meta_well_formed.
-        rewrite Hrs_key_kind_eq. rewrite <-Hrs_key_name_eq. split_and!. all: intuition. } *)
+      assert (∃ active_pure_pod, active_pure_pods !! sint.nat i = Some active_pure_pod) as [active_pure_pod Hlookup_active_pure_pods].
+      { apply lookup_lt_is_Some_2. rewrite <-Hlen2. word. }
+      iDestruct (big_sepL2_lookup_acc with "Hdeepown_pods") as "[Hdeepown_this_pod Hdeepown_other_pods]".
+      { apply Hlookup_active_pods. }
+      { apply Hlookup_active_pure_pods. }
+      assert (active_pure_pod ∈ drop (sint.nat i) active_pure_pods) as Hin_drop.
+      { apply (list_elem_of_lookup_2 _ 0). rewrite lookup_drop. rewrite Nat.add_0_r. done. }
+      set k := PurePod.key active_pure_pod.
+      assert (filter (λ kv : KKey.t * PurePod.t, is_pure_pod_active kv.2) pure_pod_map' !! k = Some active_pure_pod)
+      as Hin_filtered_pure_pod_map'.
+      { apply Hin'. done. }
+      assert (pure_pod_map' !! k = Some active_pure_pod) as Hin_pure_pod_map'.
+      { apply map_lookup_filter_Some in Hin_filtered_pure_pod_map'. intuition. }
+      assert (pure_pod_map !! k = Some active_pure_pod) as Hin_pure_pod_map.
+      { apply Hmap_sub; [done|done]. }
+      iDestruct (big_sepM_delete _ pure_pod_map' k _ Hin_pure_pod_map' with "Hghostown_pods") as "[Hghostown_this_pod Hghostown_other_pods]".
+      assert (∃ s, grand_child_keys' !! k = Some s) as [s Hin_grand_child_keys'].
+      { assert (k ∈ dom grand_child_keys') as Hin_dom.
+        { rewrite -Hdom_eq'. apply elem_of_dom. eauto. }
+        apply elem_of_dom in Hin_dom. done. }
+      iDestruct (big_sepM_delete _ grand_child_keys' k _ Hin_grand_child_keys' with "Hghostown_grandchildren")
+      as "[Hghostown_this_grandchildren Hghostown_other_grandchildren]".
+      iAssert(⌜ k = mk_pod_key (v1.ObjectMeta.Namespace' (v1.ReplicaSet.ObjectMeta' rs)) (v1.ObjectMeta.Name' (v1.Pod.ObjectMeta' active_pod)) ⌝%I) as "%Hk_eq".
+      { iNamedPrefix "Hdeepown_this_pod" "Hpod_". iNamedPrefix "Hpod_Hdeepown_objectmeta" "Hpod_". rewrite Hpod_Hdeepown_name.
+        iNamedPrefix "Hrs_Hdeepown_objectmeta" "Hrs_".
+        iPureIntro.
+        rewrite Hrs_Hdeepown_namespace. rewrite Hrs_key_namespace_eq.
+        assert(KKey.Namespace' rs_key = PureObjectMeta.Namespace' (PurePod.ObjectMeta' active_pure_pod)) as ->.
+        { symmetry. rewrite -(Hpods_ns_eq k).
+          - apply elem_of_dom. done.
+          - done. }
+        done.
+      }
+      wp_apply (wp_State__PodDelete _ _ _ _ k active_pure_pod with "[$Hghostown_this_pod $Hghostown_children $Hghostown_this_grandchildren]").
+      { iFrame "#". iPureIntro. split; [done|]. apply elem_of_dom. done. }
+      iIntros (updated_pure_pod) "H". iNamed "H". wp_auto.
+      rewrite bool_decide_true //. wp_auto.
+      iApply wp_for_post_do. wp_auto.
+      iAssert (I) with "[Hi_ptr Hpod_ptr Hghostown_other_pods Hghostown_other_grandchildren Hpod_updated_or_deleted]" as "loop_inv".
+      { iDestruct "Hpod_updated_or_deleted" as "[Hpod_updated | Hown_child_keys]".
+        - iNamed "Hpod_updated".
+          iExists (word.add i (W64 1)), this_ptr, (<[k := updated_pure_pod]> pure_pod_map'), (filter (λ kv : KKey.t * PurePod.t, is_pure_pod_active kv.2) (<[k := updated_pure_pod]> pure_pod_map')), grand_child_keys'.
+          iFrame.
+          iDestruct (big_sepM_insert _ (delete k pure_pod_map') k updated_pure_pod with "[$Hghostown_other_pods $Hown_pod]") as "Hghostown_pods".
+          { apply lookup_delete_eq. }
+          iDestruct (big_sepM_insert _ (delete k grand_child_keys') k s with "[$Hghostown_other_grandchildren $Hown_grandchild_keys]") as "Hghostown_grand_children".
+          { apply lookup_delete_eq. }
+          assert (<[k:=updated_pure_pod]> (delete k pure_pod_map') = <[k:=updated_pure_pod]> pure_pod_map') as ->.
+          { apply insert_delete_eq. }
+          assert (<[k:=s]> (delete k grand_child_keys') = grand_child_keys') as ->.
+          { rewrite insert_delete_id; done. }
+          assert (dom (<[k:=updated_pure_pod]> pure_pod_map') = dom pure_pod_map') as ->.
+          { rewrite dom_insert_lookup_L; done. }
+          iFrame. iPureIntro.
+          assert (is_pure_pod_active active_pure_pod) as Hactive.
+          { apply map_lookup_filter_Some in Hin_filtered_pure_pod_map' as [_ Hactive]. done. }
+          assert (¬ is_pure_pod_active updated_pure_pod) as Hinactive.
+          { unfold is_pure_pod_active. simpl. intro H. destruct H as (_ & _ & H). done. }
+          assert(filter (λ kv : KKey.t * PurePod.t, is_pure_pod_active kv.2) pure_pod_map !! k = Some active_pure_pod)
+          as Hin_filtered_pure_pod_map.
+          { apply map_lookup_filter_Some in Hin_filtered_pure_pod_map' as [Hlookup_k Hactive'].
+            apply map_lookup_filter_Some. split; [eapply Hmap_sub; eauto | done]. }
+          split_and!. all: try done.
+          + rewrite map_filter_insert. simpl.
+            destruct (decide (is_pure_pod_active updated_pure_pod)); [done|].
+            rewrite map_filter_delete.
+            rewrite map_size_delete_Some.
+            * done.
+            * rewrite Hpod_number'. word.
+          + intros pure_pod Hin_drop_next.
+            apply list_elem_of_lookup_1 in Hin_drop_next as [j Hlookup_j].
+            rewrite lookup_drop in Hlookup_j.
+            assert (pure_pod ∈ drop (sint.nat i) active_pure_pods) as Hin_drop_i.
+            { replace (sint.nat (word.add i (W64 1))) with (S (sint.nat i)) in Hlookup_j by word.
+              apply (list_elem_of_lookup_2 _ (S j)).
+              rewrite lookup_drop.
+              replace (S j + sint.nat i) with (j + S (sint.nat i)) by lia.
+              assert ((S (sint.nat i) + j)%nat = (sint.nat i + S j)%nat) as <- by lia.
+              done. }
+            apply Hin' in Hin_drop_i as Hlookup_k0.
+            assert (sint.nat i ≠ (sint.nat (word.add i (W64 1)) + j)%nat) as Hi_neq.
+            { word. }
+            assert (k ≠ PurePod.key pure_pod) as Hk_neq.
+            { apply (Hno_dup (sint.nat i) (sint.nat (word.add i (W64 1)) + j)%nat); [done|done|done]. }
+            rewrite map_filter_insert. simpl.
+            destruct (decide (is_pure_pod_active updated_pure_pod)); [done|].
+            rewrite map_filter_delete. rewrite lookup_delete_ne; done.
+          + intros pure_pod Hin_drop_next Hin_inserted_map'.
+            apply list_elem_of_lookup_1 in Hin_drop_next as [j Hlookup_j].
+            rewrite lookup_drop in Hlookup_j.
+            assert (pure_pod ∈ drop (sint.nat i) active_pure_pods) as Hin_drop_i.
+            { replace (sint.nat (word.add i (W64 1))) with (S (sint.nat i)) in Hlookup_j by word.
+              apply (list_elem_of_lookup_2 _ (S j)).
+              rewrite lookup_drop.
+              replace (S j + sint.nat i) with (j + S (sint.nat i)) by lia.
+              assert ((S (sint.nat i) + j)%nat = (sint.nat i + S j)%nat) as <- by lia.
+              done. }
+            apply (Hmap_sub _ Hin_drop_i).
+            assert (sint.nat i ≠ (sint.nat (word.add i (W64 1)) + j)%nat) as Hi_neq.
+            { word. }
+            assert (k ≠ PurePod.key pure_pod) as Hk_neq.
+            { apply (Hno_dup (sint.nat i) (sint.nat (word.add i (W64 1)) + j)%nat); [done|done|done]. }
+            rewrite lookup_insert_ne in Hin_inserted_map'; done.
+          + word.
+          + rewrite /slice.slice_f /=. word.
+        - iExists (word.add i (W64 1)), this_ptr, (delete k pure_pod_map'), (filter (λ kv : KKey.t * PurePod.t, is_pure_pod_active kv.2) (delete k pure_pod_map')), (delete k grand_child_keys').
+          assert (dom pure_pod_map' ∖ {[k]} = dom (delete k pure_pod_map')) as ->.
+          { rewrite dom_delete_L. done. }
+          iFrame. iPureIntro. split_and!. all: try done.
+          + rewrite !dom_delete_L. rewrite Hdom_eq'. done.
+          + rewrite map_filter_delete.
+            rewrite map_size_delete_Some.
+            * done.
+            * rewrite Hpod_number'. word.
+          + intros pure_pod Hin_drop_next.
+            apply list_elem_of_lookup_1 in Hin_drop_next as [j Hlookup_j].
+            rewrite lookup_drop in Hlookup_j.
+            assert (pure_pod ∈ drop (sint.nat i) active_pure_pods) as Hin_drop_i.
+            { replace (sint.nat (word.add i (W64 1))) with (S (sint.nat i)) in Hlookup_j by word.
+              apply (list_elem_of_lookup_2 _ (S j)).
+              rewrite lookup_drop.
+              replace (S j + sint.nat i) with (j + S (sint.nat i)) by lia.
+              assert ((S (sint.nat i) + j)%nat = (sint.nat i + S j)%nat) as <- by lia.
+              done. }
+            apply Hin' in Hin_drop_i as Hlookup_k0.
+            assert (sint.nat i ≠ (sint.nat (word.add i (W64 1)) + j)%nat) as Hi_neq.
+            { word. }
+            assert (k ≠ PurePod.key pure_pod) as Hk_neq.
+            { apply (Hno_dup (sint.nat i) (sint.nat (word.add i (W64 1)) + j)%nat); [done|done|done]. }
+            rewrite map_filter_delete. rewrite lookup_delete_ne; done.
+          + intros pure_pod Hin_drop_next Hin_inserted_map'.
+            apply list_elem_of_lookup_1 in Hin_drop_next as [j Hlookup_j].
+            rewrite lookup_drop in Hlookup_j.
+            assert (pure_pod ∈ drop (sint.nat i) active_pure_pods) as Hin_drop_i.
+            { replace (sint.nat (word.add i (W64 1))) with (S (sint.nat i)) in Hlookup_j by word.
+              apply (list_elem_of_lookup_2 _ (S j)).
+              rewrite lookup_drop.
+              replace (S j + sint.nat i) with (j + S (sint.nat i)) by lia.
+              assert ((S (sint.nat i) + j)%nat = (sint.nat i + S j)%nat) as <- by lia.
+              done. }
+            apply (Hmap_sub _ Hin_drop_i).
+            assert (sint.nat i ≠ (sint.nat (word.add i (W64 1)) + j)%nat) as Hi_neq.
+            { word. }
+            assert (k ≠ PurePod.key pure_pod) as Hk_neq.
+            { apply (Hno_dup (sint.nat i) (sint.nat (word.add i (W64 1)) + j)%nat); [done|done|done]. }
+            rewrite lookup_delete_ne in Hin_inserted_map'; done.
+          + word.
+          + rewrite /slice.slice_f /=. word.
+      }
+      iFrame.
+      iCombineNamed "Hpod_*" as "H".
+      iAssert ((this_ptr ↦{dq1} active_pod)%I) with "[H]" as "Hthis_ptr".
+      { iNamed "H". iApply (struct_fields_combine (V:=v1.Pod.t)). iFrame. }
+      iSplitL "Hthis_ptr Hother_ptrs".
+      * iApply "Hother_ptrs". done.
+      * iApply "Hdeepown_other_pods". done.
+    + iApply "HΦ". iFrame. iPureIntro. split. all: try done.
+      rewrite Hpod_number'. rewrite /slice.slice_f /= in Hi. word.
 Admitted.
 
 Lemma wp_FilterActivePods l ptrs (pods: list v1.Pod.t) dq:
@@ -298,8 +472,9 @@ Lemma wp_FilterPodsByOwner γ l owner owner_kind metadata pure_metadata dq
       PureObjectMeta.deepown_l owner metadata pure_metadata dq ∗
       parent_key [[ γ.(γ_state) ]]↦ owned_parent ∗
       ([∗ map] key ↦ pod ∈ owned_pod_map, key [[ γ.(γ_state) ]]↦ PureKObject.Pod pod) ∗
-      ⌜ ∀ key pod, owned_pod_map !! key = Some pod → PureKObject.agree_with_key key (PureKObject.Pod pod) ⌝ ∗
-      parent_key [[ γ.(γ_children) ]]↦ owned_child_keys
+      parent_key [[ γ.(γ_children) ]]↦ owned_child_keys ∗
+      ⌜ ∀ key pod, owned_pod_map !! key = Some pod → key = PurePod.key pod ⌝ ∗
+      ⌜ ∀ key, key ∈ dom owned_pod_map → key.(KKey.Namespace') = parent_key.(KKey.Namespace') ⌝
   }}}.
 Proof.
   wp_start as "H". iNamed "H". iDestruct "Hdeepown_l_meta" as "[Howner Hdeepown_meta]". subst. wp_auto.
